Update CPU model.
  - Clean up various definitions
  - Get unconditional "this-type-of-execution-unit-is-safe" lemma

Cpu.fst
@@ -14,6 +14,7 @@ type registerFile
 type systemState
      = { memory: memoryState; registers:registerFile  }
 
+(* Equivalence *)
 let equiv_system (lhs:systemState) (rhs:systemState)
     =    (lhs.registers.pc = rhs.registers.pc)
        /\ (equiv  lhs.registers.value rhs.registers.value)
@@ -34,12 +35,7 @@ let system_equivalence_is_symmetric (lhs rhs:systemState):
       list_equivalence_is_symmetric _ lhs.memory          rhs.memory
 
 
-let equal (lhs:systemState) (rhs:systemState)
-    =   (lhs.registers.pc = rhs.registers.pc)
-       /\ (lhs.registers.value = rhs.registers.value)
-       /\ (lhs.memory = rhs.memory)
-
-
+(* Redaction *)
 let redact_system (s:systemState): systemState = {
                                        registers = { s.registers with value = redact s.registers.value 0 };
                                        memory    = redact_list s.memory 0
@@ -56,22 +52,14 @@ let equivalent_systems_have_equal_redactions (s1:systemState) (s2:systemState):
     = equivalent_values_have_equal_redactions _ s1.registers.value s2.registers.value 0;
       equivalent_lists_have_equal_redactions  _ s1.memory s2.memory 0
 
-      (*
-let _ = assert(forall (s1:systemState) (s2:systemState) (f: systemState -> systemState).
-                 (equal s1 s2) ==> (let t1, t2 = f s1, f s2 in (
-                          (s1.registers.pc    == s2.registers.pc)
-                        /\ (s1.registers.value == s2.registers.value)
-                        /\ (t1.registers.pc    == t2.registers.pc)
-                        /\ (t1.registers.value == t2.registers.value)
-                          (equal (f s1) (f s2))
-                 ))
-              )
 
-   *)
-      (*
-let _ = assert(forall (x y z: systemState). ( (equal x y) /\ (equal y z) ==> (equal x z)) )
-  *)
-
+(*******************************************************************************
+ * System definition.
+ *
+ * We build our system from an execution unit (essentially, an ISA)
+ * and a function that "steps" the processor state (essentially, the
+ * microarchitecture, which for now just fetch-executes in a single step).
+ *)
 type execution_unit = word -> systemState -> systemState
 
 val step
@@ -85,63 +73,63 @@ let step exec pre_state =
         | Blinded _ -> pre_state
         | Clear inst -> exec inst pre_state
 
-let is_safe_single_step (exec:execution_unit) (pre:systemState) =
-    (equiv_system (step exec pre) (step exec (redact_system pre)))
-
-let is_safe_execution_unit_single_step (exec:execution_unit) =
-        forall (pre:systemState). is_safe_single_step exec pre
-
-let all_single_steps_safe_mean_execution_unit_is_safe  (exec:execution_unit):
-    Lemma (requires forall (pre:systemState). (is_safe_single_step exec pre))
-          (ensures  is_safe_execution_unit_single_step exec)
-          = ()
-
-
-type single_step_safe_execution_unit = e:execution_unit{is_safe_execution_unit_single_step e}
-
+(*******************************************************************************
+ * Equivalence-based safety.
+ *
+ * We define safety in this case to be that the system is safe if executing on
+ * equivalent (and so indistinguishable) states always results in equivalent
+ * output states.
+ *******************************************************************************)
 let equivalent_inputs_yield_equivalent_states (exec:execution_unit) (pre1 pre2 : systemState) =
-            equiv_system pre1 pre2 ==> equiv_system (step exec pre1) (step exec pre2)
+    equiv_system pre1 pre2 ==> equiv_system (step exec pre1) (step exec pre2)
 
 let is_safe (exec:execution_unit) =
-  forall (pre1 pre2 : systemState). equivalent_inputs_yield_equivalent_states exec pre1 pre2
-
+    forall (pre1 pre2 : systemState). equivalent_inputs_yield_equivalent_states exec pre1 pre2
 
 type safe_execution_unit = exec:execution_unit{is_safe exec}
 
-let single_step_safe_execution_units_give_equivalent_outputs_for_equivalent_inputs
-    (exec:execution_unit) (pre_1:systemState) (pre_2:systemState)
-    : Lemma (requires (is_safe_execution_unit_single_step exec) /\ equiv_system pre_1 pre_2)
-            (ensures equiv_system (step exec pre_1) (step exec pre_2))
-      = equivalent_systems_have_equal_redactions pre_1 pre_2;
+(*******************************************************************************
+ * Redacting-equivalent execution units.
+ *
+ * We can show that a system constructed from an execution unit that produces
+ * an equivalent output when operating on the same input but with the blinded
+ * values zeroed is safe.
+ *******************************************************************************)
+
+type redacting_equivalent_execution_unit
+   = exec:execution_unit{
+     forall(pre:systemState) (inst:word).  (equiv_system (exec inst pre) (exec inst (redact_system pre))) }
+
+let is_redacting_equivalent_system_single_step_somewhere (exec:execution_unit) (pre:systemState) =
+    (equiv_system (step exec pre) (step exec (redact_system pre)))
+
+let is_redacting_equivalent_system_single_step_everywhere (exec:execution_unit) =
+    forall (pre:systemState). is_redacting_equivalent_system_single_step_somewhere exec pre
+
+let redacting_equivalent_execution_units_lead_to_redacting_equivalent_systems_somewhere
+    (exec:redacting_equivalent_execution_unit) (pre:systemState):
+    Lemma (ensures is_redacting_equivalent_system_single_step_somewhere exec pre) =
+      let redaction = redact_system pre in
+      systems_are_equivalent_to_their_redaction pre;
+      assert(pre.registers.pc = redaction.registers.pc);
+      let pc = pre.registers.pc in
+      equivalent_memories_have_equivalent_values pre.memory redaction.memory pc
+
+let redacting_equivalent_systems_give_equivalent_outputs_for_equivalent_inputs
+    (exec:redacting_equivalent_execution_unit) (pre_1:systemState) (pre_2:systemState)
+      : Lemma (requires equiv_system pre_1 pre_2)
+              (ensures equiv_system (step exec pre_1) (step exec pre_2))
+              [SMTPat (equiv_system (step exec pre_1) (step exec pre_2))]
+      = redacting_equivalent_execution_units_lead_to_redacting_equivalent_systems_somewhere exec pre_1;
+        redacting_equivalent_execution_units_lead_to_redacting_equivalent_systems_somewhere exec pre_2;
+        equivalent_systems_have_equal_redactions pre_1 pre_2;
         assert( (step exec (redact_system pre_1)) == (step exec (redact_system pre_2)) );
         system_equivalence_is_symmetric (step exec pre_2) (step exec (redact_system pre_2));
         assert( equiv_system (step exec (redact_system pre_2)) (step exec pre_2) );
         system_equivalence_is_transitive (step exec pre_1) (step exec (redact_system pre_1)) (step exec pre_2)
 
-let single_step_safe_execution_units_are_safe
-      (exec:single_step_safe_execution_unit):
-      Lemma (ensures is_safe exec)
-      = assert( is_safe_execution_unit_single_step exec ) ;
-        assert( forall (pre:systemState). is_safe_single_step exec pre ) ;
-        assert( forall (pre1:systemState) (pre2: systemState{equiv_system pre1 pre2}). (equiv_system (step exec pre1) (step exec pre2)))
+let redacting_equivalent_execution_units_are_safe
+    (exec:redacting_equivalent_execution_unit):
+    Lemma (ensures is_safe exec)
+      = ()
 
-
-(* Now let's look at what the execution units should look like. *)
-type redacting_execution_unit = exec:execution_unit{
-     forall (inst:word) (pre:systemState). (equiv_system (exec inst pre) (exec inst (redact_system pre)))}
-
-
-let redacting_execution_unit_is_everywhere_safe (pre1 pre2 : systemState) (exec:redacting_execution_unit):
-  Lemma (requires equiv_system pre1 pre2)
-        (ensures equiv_system (step exec pre1) (step exec pre2))
-  = equivalent_systems_have_equal_redactions pre1 pre2;
-    assert( (step exec (redact_system pre1)) == (step exec (redact_system pre2)) );
-    assert( equiv_system (step exec pre2) (step exec (redact_system pre2)) ) ;
-                                                admit() ;
-    system_equivalence_is_symmetric (step exec pre2) (step exec (redact_system pre2));
-    assert( equiv_system (step exec (redact_system pre2)) (step exec pre2) );
-    system_equivalence_is_transitive (step exec pre1) (step exec (redact_system pre1)) (step exec pre2)
-
-let redacting_execution_unit_is_single_step_safe (exec:redacting_execution_unit)
-  : Lemma (ensures is_safe exec)
-  = ()
